Clean.lean
@@ -1,3 +1,4 @@
+import Clean.Caliper.MultiLimbCompile
 import Clean.Caliper.MultiLimb
 import Clean.Caliper.WitgenCompile
 import Clean.Caliper.WitgenComputable
